---
title: "Arrow's Impossiblity Theorem"
author: "~sambex-fadsen"
output: html_document
---
```{r setup, include=FALSE}
knitr::opts_chunk$set(echo = FALSE,fig.align='center')
```
<style>
body {
    background-color: #333;
    color: #FFFFFF;
}
</style>

### 3 Reasonable Demands

Let's start with some definitions. Given $n$ voters $\{x_1,x_2...,x_n\}$ and $m$ candidates $\{y_1,y_2...,y_m\}$, we define $\mathcal{O}$ to be the set of all $m!$ _order preferences_ over our candidates. 

A _preference profile_ is an element $\theta \in \mathcal{O}^n$, where we let $\theta_i$ be the order preference of the $i$th voter. In particular, we write $\theta_i(a) \succ \theta_i(b)$ if voter $x_i$ prefers candidate $y_a$ to candidate $y_b$.

Finally, a _social aggregation function_ is any function $f: \mathcal{O}^n \to \mathcal{O}$ which maps a given preference profile to a unique order preference (you can think of this as our 'voting system').

Now, we are ready to describe the 3 demands we want our social aggregation function $f$ to satisfy. I will define each demand formally and then use plain English to make each one seem reasonable.

First, $f$ satisfies _unanimity_ iff $\forall \theta \in \mathcal{O}^n$:
$$(\forall i \in [n], \ \theta_i(a) \succ \theta_i(b)) \implies  f(\theta)(a) \succ f(\theta)(b)$$
This means if each of our voters prefers $y_a$ to $y_b$, then the aggregate preference must also favor $y_a$ to $y_b$.

Second, $f$ satisfies _binary independence_ iff $\forall \theta,\tau \in \mathcal{O}^n$:
$$(\forall i \in [n], \ \theta_i(a) \succ \theta_i(b) \leftrightarrow \tau_i(a) \succ \tau_j(b)) \implies (f(\theta)(a) \succ f(\theta)(b) \leftrightarrow f(\tau)(a) \succ f(\tau)(b) )$$
In other words, the aggregate preference between $y_a$ and $y_b$ is uniquely determined by each voter's preference between $y_a$ and $y_b$.

Third, $f$ satisfies _non-dictatorship_ iff:
$$\neg(\exists i \in [n] \ \text{s.t.} \ \forall \theta \in \mathcal{O}, \ f(\theta)=\theta_i)$$
That is to say, there does not exist a voter whose order preference is _always_ the aggregate preference.

Hopefully, these demands seem like sensible things to ask from a voting system. If they don't, maybe try convincing yourself that a simple majority rule procedure between two candidates _does_ satisfy them.

Unfortunately, when there are more than $2$ candidates, turns out we're asking for too much...

### Proof of the Theorem
STAC there exists a social aggregation function $f$ satisfying unanimity, binary independence, and non-dictatorship in an election with more than 2 candidates...

#### Defining Pivots
Given two candidates $y_a$, $y_b$, we define the _pivot_ from $a$ to $b$ as follows.

Consider a preference profile $\theta^0 \in \mathcal{O}^n$ where $\forall i \in [n]$:
$$\theta^0_i(a) \succ \theta^0_i(b)$$
By unanimity, we must have:
$$f(\theta^0)(a) \succ f(\theta^0)(b)$$
Now pick $\theta^{k} \in \mathcal{O}^n$ so that $\forall i \in [n]\backslash [k]$:
$$\theta^{k}_i(a) \succ \theta^{k}_i(b)$$
but $\forall i \in [k]$:
$$\theta_i^{k}(a) \prec \theta_i^{k}(b) $$
In particular, the last preference profile $\theta^n$ will have $\forall i \in [n]$:
$$\theta^n_i(a) \prec \theta^n_i(b)$$
Thus by unanimity, we must have:
$$f(\theta^n)(a) \prec f(\theta^n)(b)$$
Moreover, we are guarenteed the existence of an integer $b|a \in [n]$ satisfying:
$$b|a=\min\{k \ | \ f(\theta^k)(a) \prec f(\theta^k)(b) \}$$
We call the candidate $x_{b|a}$ our "pivot" from $a$ to $b$.  Note $b|a$ is _unique_ despite our particular choice of $\theta^0,\theta^1...,\theta^n$ since $f$ satisfies binary independence. 

Additionally, if $\theta \in \mathcal{O}^n$ is a preference profile so that $\forall i \in [1, b|a)$:
$$\theta_i(a) \succ \theta_i(b)$$
and $\forall i \in (b|a,n]$:
$$\theta_i(a) \prec \theta_i(b)$$
then by construction:
$$f(\theta)(b) \succ f(\theta)(a) \iff \theta_{b|a}(b) \succ \theta_{b|a}(a)$$

#### The Power of Pivots
Let's introduce a third candidate $y_c$ and suppose we have a preference profile $\tau \in \mathcal{O}^n$ so that  $\forall i \in [1, b|a]$:
$$\tau_i(a) \succ \tau_i(b) \succ \tau_i(c) $$
, and $\forall i \in (b|a,n]$:
$$\tau_i(a) \prec \tau_i(c) \prec \tau_i(b)$$
Since $b|a$ is the pivot from $a$ to $b$, we know that:
$$f(\tau)(a) \succ f(\tau)(b)$$
Also by unanimity:
$$f(\tau)(b) \succ f(\tau)(c)$$
Thus:
$$f(\tau)(a) \succ f(\tau)(b) \succ f(\tau)(c)$$
Now, if voter $x_{b|a}$ switches their order preference so:
$$\tau_{b|a}(b) \succ \tau_{b|a}(a) \succ \tau_{b|a}(c) $$
and the rest of the voters arbitrarily shuffle their preferences between $y_b$ and $y_c$, then binary independence implies we still have:
$$f(\tau)(a) \succ f(\tau)(c)$$
Moreover, since $b|a$ is the pivot from $a$ to $b$:
$$f(\tau)(b) \succ f(\tau)(a)$$
Thus:
$$f(\tau)(b) \succ f(\tau)(a) \succ f(\tau)(c)$$
Finally, if all the voters arbitrarily change their ranking of $y_a$, then binary independence implies we still have:
$$f(\tau)(b)  \succ f(\tau)(c)$$
Thus, so long as voter $x_{b|a}$ prefers candidate $y_b$ to $y_c$, this dictates $f(\tau)(b) \succ f(\tau)(c)$, _regardless of everyone else's preferences_. 

In other words the pivot from $a$ to $b$ gets to force all candidates (except for $y_a$) below $y_b$ in the aggregate preference if they so chose. Interesting, nâ€™est ce pas? 

#### All Pivots are the Same

Consider a preference profile $\theta \in \mathcal{O}^n$ such that $\forall i \in [1,b|a)$:
$$\theta_i(b) \succ \theta_i(c)$$
and $\forall i \in (b|a,n]$:
$$\theta_i(c) \succ \theta_i(b)$$
As we saw at the end of the last section, since $\theta_{b|a}(b) \succ \theta_{b|a}(c)$ we must have:
$$f(\theta)(b) \succ f(\theta)(c)$$
Thus $b|c \leq b|a$.

Now consider a preference profile $\theta \in \mathcal{O}^n$ such that $\forall i \in [1,b|a)$:
$$\theta_i(c) \succ \theta_i(b)$$
and $\forall i \in [b|a,n]$:
$$\theta_i(b) \succ \theta_i(c)$$
As we saw at the end of the last section, since $\theta_{b|a}(b) \succ \theta_{b|a}(c)$ we must have:
$$f(\theta)(b) \succ f(\theta)(c)$$
Thus $c|b \geq b|a$. Putting this together with the previous inequality:
$$b|c \leq b|a \leq c|b$$
By symmetry we have:
$$c|b \leq c|a \leq b|c$$
Thus:
$$b|c=c|b=a|b=b|a=c|a=a|c$$
Since all pivots are the same, there exists a voter who gets to force each candidate below any other candidate in the aggregate preference. Thus this voter is a dictor, contradicting our assumption that $f$ is non-dictatorial!

### Probabilistic Arrow's Theorem

Now that we've seen the proof of Arrow's theorem proper, I want to look at a slightly tweaked version! 

Instead of aggregating a group of individuals' preference orders over of set of candidates, we are now going to aggregate their _probability distributions_ over a measurable space $(\Omega, \mathcal{F})$.

We require $\Omega$ contain more than 2 measurable outcomes (this is analagous to having more than $2$ candidates). Also, we will denote the set of all possible measures over $(\Omega, \mathcal{F})$ by $\mathcal{M}$. 

In particular, the probability distributions of our $n$ individuals will be characterized by a _opinion pool_ $\{P_1, P_2, ...P_n\} \in \mathcal{M}^n$. 

A _consensus function_ will be a function $C: \mathcal{M}^n \to \mathcal{M}$ which maps a given opinion pool to a unique probability distribution over $(\Omega, \mathcal{F})$.

Once again, we have three seemingly reasonable demands:

First, $C$ satisfies the _independence preservation property_ (IPP) iff :
$$(\forall i \in [n], \ P_i(A \cap B)=P_i(A)\cdot P_i(B)) \implies C(P_1,P_2,...P_n)(A\cap B)=C(P_1,P_2,...P_n)(A)\cdot C(P_1,P_2,...P_n)(B)$$
IPP parallels our previous notion of _unanimity_ in that if each individual thinks events $A$ and $B$ are independent, then the aggregate distribution also treats $A$ and $B$ as independent. 

Second, $C$ satisfies the _strong setwise function property_ (SSFP) iff $\exists G: [0,1]^n \to [0,1]$ such that for any given opinion pool $\{P_1,P_2,...,P_n\}\in \mathcal{M}^n$:
$$\forall A \in \mathcal{F}, \ C(P_1, P_2, ...P_n)(A)=G(P_1(A),P_2(A),...P_n(A))$$
SSFP is analagous to _binary independence_ since it implies the aggregate probability of a given event is uniquely determined by the probabilities each individual assigns to that event.

Third, $C$ satisfies _non-dictatorship_ iff:
$$\neg(\exists i \in [n] \ \text{s.t.} \ \forall \{P_1,P_2,...,P_n\}\in \mathcal{M}^n, \ \forall A \in \mathcal{F}, \ C(P_1,P_2,...P_n)(A)=P_i(A) )$$
As before, we will proceed by showing IPP + SSFP necessarily violate non-dictatorship.

However, we need to first establish a crucial and somewhat surprising lemma...

#### SSFP $\iff$ Consensus is Linear

We claim $C$ satisfies SSFP iff $\exists w_1, w_2,...w_n \in [0,1]$ such that $\sum_{i=1}^n w_i=1$ and for any given opinion pool $\{P_1,P_2,...P_n\}\in \mathcal{M}^n$,  $\forall A \in \mathcal{F}$:
$$C(P_1,P_2,...P_n)(A)=G(P_1(A),P_2(A),...P_n(A))=\sum_{i=1}^n w_i \cdot P_i(A)$$
 
**Proof:**
\
It trivially follows that linear consensus $\implies$ SSFP so we will only show the other direction.

Consider three disjoint non-empty subsets $A, B, C \in \mathcal{F}$ which partition $\Omega$ (we are guarenteed these exist by the assumption $\Omega$ has more than 2 measurable outcomes).

Let $(a_1,b_1),(a_2,b_2),...(a_n,b_n) \in \mathbb{R}^2_{\geq 0}$ so that $\forall i \in [n], \ a_i+b_i \leq 1$. We construct an opinion pool $\{P'_1, P'_2, ... P'_n\} \in \mathcal{M}^n$ so that:
\begin{align*}
&P'_i(A)=a_i
\\
&P'_i(B)=b_i
\\
&P'_i(C)=1-(a_i+b_i)
\end{align*}
By SSFP:
\begin{align*}
G(a_1+b_1,a_2+b_2,...a_n+b_n)&=G(P'_1(A)+P'_1(B),P'_2(A)+P'_2(B),...P'_n(A)+P'_n(B))
\\
&=G(P'_1(A\cup B),P'_2(A\cup B),...P'_n(A\cup B))
\\
&=C(P'_1,P'_2,...P'_n)(A \cup B)
\\
&=C(P'_1,P'_2,...P'_n)(A)+C(P'_1,P'_2,...P'_n)(B)
\\
&=G(P'_1(A),P'_2(A),...P'_n(A))+G(P'_1(B),P'_2(B),...P'_n(B))
\\
&=G(a_1,a_2,...a_n)+G(b_1,b_2,...b_n)
\end{align*}

In particular, this implies $\forall x=\{x_1,x_2,...x_n\}\in [0,1]^n$:
\begin{align*}
G(x_1,x_2,...x_n)=G(x_1,0,...0)+G(0,x_2,...x_n)=\sum_{i=1}^n G(0,...0,x_i,0,...0)
\end{align*}
More concisely, if we write $G_i(a)=G(\underbrace{0,...0}_{i-1\ 0's},a,0,...0)$ then:
$$G(x)=\sum_{i=1}^n G_i(x_i)$$
Now if $a,b \in [0,1]$ so that $a+b \in [0,1]$, then from before:
\begin{align*}
G_i(a+b)&=G(0,...0,a+b,0,...0)
\\
&=G(0,...0,a,0,...0)+G(0,...0,b,0,...0)
\\
&=G_i(a)+G_i(b)
\end{align*}
, i.e. each $G_i$ satisfies the Cauchy functional equation on the unit interval. Note $\forall n \in \mathbb{N}^+$:
$$G_i(x)=G_i\left(\frac{n}{n}\cdot x\right)=n\cdot G_i\left(\frac{x}{n}\right)$$
, i.e.
$$\frac{1}{n}\cdot G_i(x)=G_i\left(\frac{x}{n}\right)$$
Now if $m\in \mathbb{N}_{\geq 0}$ so that $\frac{m}{n} \in \mathbb{Q}_{\geq 0} \cap [0,1]$ then:
$$G_i\left(\frac{m}{n}\cdot x\right)=m\cdot G_i\left(\frac{x}{n}\right)=\frac{m}{n}\cdot G_i(x)$$
Finally $\forall r \in [0,1]$ can pick a rational $q_r \in [0,1]$ arbitrarily close so that $d_r=r-q_r \in [0,\frac{1}{N}]$ for any given $N \in \mathbb{N}$. Note:
\begin{align*}
G_i(r)-G_i(1)\cdot r&=G_i(r-q_r+q_r)-G_i(1)\cdot r
\\
&=G_i(r-q_r)+G_i(q_r)-G_i(1)\cdot r
\\
&=G_i(r-q_r)+(q_r-r)\cdot G_i(1)
\\
&=G_i(d_r)-d_r\cdot G_i(1)
\end{align*}
We know $\text{Im}(G_i)\subseteq [0,1]$ as its values must be probabilities. Thus $G_i(d_r)\leq \frac{1}{N}$ (otherwise $G_i(N \cdot d_r)=N \cdot G_i(d_r) > 1$) and $G_i(1) \leq 1$. Hence:
$$|G_i(r)-G_i(1)\cdot r|=|G_i(d_r)-d_r\cdot G_i(1)|\leq |G_i(d_r)|+d_r\cdot|G_i(1)| \leq \frac{2}{N}$$
Taking the limit as $N \to \infty$ yields:
$$G_i(r)=G_i(1)\cdot r$$
Thus $\forall i \in [n]$, $G_i$ is of the form:
$$G_i(x)=w_i \cdot x$$
where $w_i \in [0,1]$.

Putting things together, this implies for any given opinion pool $\{P_1,P_2,...P_n\} \in \mathcal{M}^n$, $\forall A \in \mathcal{A}$:
\begin{align*}
C(P_1,P_2,...P_n)(A)&=G(P_1(A),P_2(A),...P_n(A))
\\
&=\sum_{i=1}^n G_i(P_i(A))
\\
&=\sum_{i=1}^n w_i \cdot P_i(A)
\end{align*}

In particular, when $A=\Omega$ we have:
$$1=C(P_1,P_2,...P_n)(\Omega)=\sum_{i=1}^n w_i \cdot P_i(\Omega)=\sum_{i=1}^n w_i$$
as desired. Phew! $\square$

#### IPP + SSFP $\implies$ Dictatorship
As before, consider three disjoint non-empty subsets $A, B, C \in \mathcal{F}$ which partition $\Omega$. By the above, SSFP implies $\exists w_1,w_2...w_n \in [0,1]$ summing to $1$ so that for any given opinion pool $\{P_1,P_2,...P_n\}\in \mathcal{M}^n$:

\begin{align*}
&C(P_1,P_2,...P_n)(A)=\sum_{i=1}^n w_i P_i(A)
\\
&C(P_1,P_2,...P_n)(B)=\sum_{i=1}^n w_i P_i(B)
\\
&C(P_1,P_2,...P_n)(C)=\sum_{i=1}^n w_i P_i(C)
\end{align*}

Since not all $w_i$ can be zero we know $\exists k \in [n]$ so that $w_k>0$. We construct an opinion pool $\{P'_1,P'_2,...P'_n\}$ so that:
$$\left(P'_k(A),\ P'_k(B), P'_k(C)\right)=\left(0,\frac{1}{2},\frac{1}{2} \right)$$
and $\forall i \in [n] \backslash \{k\}$:
$$\left(P'_i(A),\ P'_i(B), P'_i(C)\right)=\left(\frac{1}{2},\frac{1}{2},0 \right)$$
Note:
\begin{align*}
&C(P'_1,P'_2,...P'_n)(A)=\frac{1-w_k}{2}
\\
&C(P'_1,P'_2,...P'_n)(B)=\frac{1}{2}
\\
&C(P'_1,P'_2,...P'_n)(C)=\frac{w_k}{2}
\end{align*}

Consider the events $S=A \cup B$ and $T=B \cup C$. By the above:
\begin{align*}
&C(P'_1,P'_2,...P'_n)(S)=\frac{1-w_k}{2}+\frac{1}{2}=1-\frac{w_k}{2}
\\
&C(P'_1,P'_2,...P'_n)(T)=\frac{1}{2}+\frac{w_k}{2}
\end{align*}

Since $P'_k(S)=P'_k(A)+P'_k(B)=\frac{1}{2}$ and $P'_k(T)=P'_k(B)+P'_k(C)=1$:
$$P'_k(S \cap T)=P'_k(B)=\frac{1}{2}=\frac{1}{2}\cdot 1=P'_k(S) \cdot P'_k(T)$$
Additionally, since  $\forall i \in [n] \backslash \{k\}$, $P'_i(S)=P'_i(A)+P'_i(B)=1$ and $P'_i(T)=P'_i(B)+P'_i(C)=\frac{1}{2}$: 
$$P'_i(S \cap T)=P'_i(B)=\frac{1}{2}=1\cdot \frac{1}{2}=P'_i(S) \cdot P'_i(T)$$
Thus by IPP, we must have:
$$C(P'_1,P'_2,...P'_n)(B)=C(P'_1,P'_2,...P'_n)(S \cap T)=C(P'_1,P'_2,...P'_n)(S) \cdot C(P'_1,P'_2,...P'_n)(T)$$
Hence:
$$\frac{1}{2}=\left(1-\frac{w_k}{2}\right)\cdot \left(\frac{1}{2}+\frac{w_k}{2}\right)$$
The only solutions to the above quadratic are $w_k=0$ and $w_k=1$. However, $w_k>0$ by assumption, implying $w_k=1$ and all other $w_i=0$. This means for any given opinion pool $\{P_1,P_2,...P_n\}\in \mathcal{M}^n$, $\forall A \in \mathcal{F}$:
$$C(P_1,P_2,...P_n)(A)=\sum_{i=1}^n w_i \cdot P_i(A)=P_k(A)$$
In other words, we have found our dictator! Thus, given more than 2 measurable outcomes, _no_ consensus function can satisfy IPP, SSFP, and non-dictatorship simultaneously :)